line.thy
@@ -124,8 +124,11 @@ definition leftPSegment :: "point2d \<Rightarrow> point2d \<Rightarrow> point2d"
   "xCoord A \<noteq> xCoord B \<Longrightarrow> leftPSegment A B \<equiv> (if (leftFromPoint A B) then A else B)"
 definition rightPSegment :: "point2d \<Rightarrow> point2d \<Rightarrow> point2d" where
   "xCoord A \<noteq> xCoord B \<Longrightarrow> rightPSegment A B \<equiv> (if (leftFromPoint A B) then B else A)"
+
 definition pointAboveSegment :: "point2d \<Rightarrow> point2d \<Rightarrow> point2d \<Rightarrow> bool" where
   "segment A B \<Longrightarrow> pointAboveSegment p A B \<equiv> yCoord p > yCoord A \<or> yCoord p > yCoord B"
+definition pointBelowSegment :: "point2d \<Rightarrow> point2d \<Rightarrow> point2d \<Rightarrow> bool" where
+  "segment A B \<Longrightarrow> pointBelowSegment p A B \<equiv> yCoord p < yCoord A \<or> yCoord p < yCoord B"
 
 (*Zusätliche Lemmas*)
 lemma intersectNotCollinear: "segment a b \<Longrightarrow> segment c d \<Longrightarrow> intersect a b c d \<Longrightarrow>
